\item {Proof: } From 
\eqref{eq:8.5.49_constr_a},
\eqref{eq:8.5.49_constr_c},
\eqref{eq:8.5.49_constr_d} and 
\eqref{eq:8.5.49_constr_e}
\begin{align}
\vec{C}-\vec{E} &= r \myvec{1 + \cos\brak{\frac{\alpha+\beta}{2}}\\ -\sin \brak{\frac{\alpha+\beta}{2}}}
\\
&= 2r \cos\brak{\frac{\alpha+\beta}{4}} \myvec{\cos\brak{\frac{\alpha+\beta}{4}}\\ -\sin \brak{\frac{\alpha+\beta}{4}}} \quad \text{ and }
\label{eq:8.5.49_ce}
\\
\norm{\vec{C}-\vec{E}} &= 2r \cos\brak{\frac{\alpha+\beta}{4}}
\label{eq:8.5.49_cenorm}
\end{align}
and 
\begin{align}
\vec{A}-\vec{D} &= r \myvec{\cos \beta + \cos\brak{\frac{\alpha-\beta}{2}}\\ -\sin \beta+\sin \brak{\frac{\alpha-\beta}{2}}}
\\
&= 2r \cos\brak{\frac{\alpha+\beta}{4}} \myvec{ \cos \brak{\frac{\alpha-3\beta}{4}} \\ \sin \brak{\frac{\alpha-3\beta}{4}}} \text{ and }
\label{eq:8.5.49_ad}
\\
\norm{\vec{A}-\vec{D}} &= 2r \cos\brak{\frac{\alpha+\beta}{4}}
\label{eq:8.5.49_adnorm}
\end{align}
Thus, 
\begin{align}
\cos \phase{B} &= \frac{\brak{\vec{A}-\vec{D}}\brak{\vec{C}-\vec{E}}}{\norm{\vec{A}-\vec{D}}\norm{\vec{C}-\vec{E}}}
\\
&= \cos \brak{\frac{\alpha-\beta}{2}}
\\
\implies \phase{B} &= \frac{\alpha-\beta}{2}
\end{align}
%
upon substituting from \eqref{eq:8.5.49_ad},
\eqref{eq:8.5.49_adnorm},
\eqref{eq:8.5.49_ce},
\eqref{eq:8.5.49_cenorm} and simplifying.

