\item {\em Proof: }Let 
\begin{align}
\vec{F} &= \frac{{{m\vec{C}} +\vec{B}}}{m+1}
\end{align}
%
From \eqref{eq:8.1.47_constr_e}
\begin{align}
\vec{E} &= \frac{{{k\vec{D}} +\vec{A}}}{k+1}
\\
\implies \vec{E} - \vec{F} &= \frac{{{k\vec{D}} +\vec{A}}}{k+1}-\frac{{{m\vec{C}} +\vec{B}}}{m+1}
\label{eq:8.1.47_sol_EF}
\\
& = \frac{\vec{A}}{k+1}-\frac{{{m\vec{C}} +\vec{B}}}{m+1}
\label{eq:8.1.47_sol_EF2}
\end{align}
$\because D = \vec{0}$.
\begin{align}
\because AB &\parallel BC, 
\\
\vec{C}-\vec{D} &= l\brak{\vec{B}-\vec{A}}
\\
\implies \vec{C} &= l\brak{\vec{B}-\vec{A}}
\label{eq:8.1.47_sol_C}
\end{align}
%
Substituting \eqref{eq:8.1.47_sol_C} in \eqref{eq:8.1.47_sol_EF2},
\begin{align}
 \vec{E} - \vec{F} &= \frac{\vec{A}}{k+1}-\frac{{{ml\brak{\vec{B}-\vec{A}}} +\vec{B}}}{m+1}
\\
 &= \vec{A}\brak{\frac{1}{k+1} + \frac{lm}{m+1}} - \vec{B}\brak{\frac{ml+1}{m+1}}
\label{eq:8.1.47_sol_EFinAB}
\end{align}
But $ EF \parallel AB$. So, for some w
\begin{align}
\implies \vec{E} - \vec{F} = w\brak{\vec{A}-\vec{B}}
\label{eq:8.1.47_sol_EFinAB2}
\end{align}
%
Comparing \eqref{eq:8.1.47_sol_EFinAB2} and \eqref{eq:8.1.47_sol_EFinAB}. We have
\begin{align}
\frac{1}{k+1} + \frac{lm}{m+1} &= \frac{ml+1}{m+1} = w
\\
\implies m+1+\brak{k+1}lm &= \brak{lm+1}\brak{k+1} 
\label{eq:8.1.47_sol_sol}
\\
\text{or, } m &=k
\end{align}
