From \eqref{eq:8.5.43_constr_b} - \eqref{eq:8.5.43_constr_d}
\begin{align}
\vec{B} - \vec{A} &= \myvec{b\\0}\label{eq:8.5.43_dir1}\\
\vec{D} - \vec{C} &= \myvec{2h\cot{\theta}-b\\0}\label{eq:8.5.43_dir2}\\
\vec{D} - \vec{A} &= \myvec{h\cot{\theta}\\h}\label{eq:8.5.43_dir3}\\
\vec{B} - \vec{C} &= \myvec{h\cot{\theta}\\-h}\label{eq:8.5.43_dir4}
\end{align}

Finding the scalar products:
\begin{align}
\brak{\vec{D} - \vec{A}}^T\brak{\vec{B} - \vec{A}} &= \norm{\vec{D}-\vec{A}} 
\norm{ \vec{B}-\vec{A}} \cos{\theta}\label{eq:8.5.43_scalar1}\\
\brak{\vec{D} - \vec{C}}^T\brak{\vec{B} - \vec{C}} &= \norm{\vec{D}-\vec{C}} 
\norm{ \vec{B}-\vec{C}} \cos{\alpha}\label{eq:8.5.43_scalar2}
\end{align}

Dividing \eqref{eq:8.5.43_scalar2} with \eqref{eq:8.5.43_scalar1},
\begin{align}
\frac{\brak{\vec{D} - \vec{A}}^T\brak{\vec{B} - \vec{A}}}{\brak{\vec{D} - \vec{C}}^T\brak{\vec{B} - \vec{C}}} &= \frac{\norm{\vec{D}-\vec{A}}\ 
\norm{ \vec{B}-\vec{A}} \cos{\theta}}{\norm{\vec{D}-\vec{C}} 
\norm{ \vec{B}-\vec{C}} \cos{\alpha}}\label{eq:8.5.43_scalar3}
\end{align}\\
$\because \norm{ \vec{D} - \vec{A} } = \norm{ \vec{B} - \vec{C}} $, \eqref{eq:8.5.43_scalar3} can be simplified to the form
\begin{align}
\frac{\brak{\vec{D} - \vec{A}}^T\brak{\vec{B} - \vec{A}}}{\brak{\vec{D} - \vec{C}}^T\brak{\vec{B} - \vec{C}}} &= \frac{\norm{ \vec{B}-\vec{A}} \cos{\theta}}{\norm{\vec{D}-\vec{C}}cos{\alpha}}
\end{align}
%
Substituting values from \eqref{eq:8.5.43_dir1}, \eqref{eq:8.5.43_dir2}, \eqref{eq:8.5.43_dir3} and \eqref{eq:8.5.43_dir4}:
\begin{align}
\frac{bh\cot{\theta}}{\brak{2h\cot{\theta}-b}h\cot{\theta}} &= \frac{b\cos{\theta}}{b-2h\cot{\theta}}\\
\implies\cos{\alpha} &= -\cos{\theta}\\
\implies \alpha + \theta &= 180\degree
\end{align}

$\therefore ABCD$ is a cyclic quadilateral.
