\item {\em Proof: } 
%\begin{multline}
% \brak{\vec{D}-\vec{B}}^T\brak{\vec{C}-\vec{A}} 
%\\
%=r^2\myvec{\cos \theta_1+1 & \sin \theta_1  }\myvec{\cos \theta-1 & \sin \theta  }
%\\
%=r^2\brak{\cos \brak{\theta_1- \theta} + \cos \theta_1 - \cos \theta -1  }
%\\
%=r^2 \brak{\cos \theta_1 - \cos \theta -\frac{1}{2} }
%\end{multline}
%$\because \theta_1-\theta = 60 \degree$. Also, using the cosine formula in $\triangle s OBD$ and $OCA$,
\begin{align}
\vec{D}-\vec{B}&= r\myvec{\cos \theta_1+1 & \sin \theta_1  } 
\\
&= 2r \cos\brak{\frac{\theta_1}{2}} \myvec{\cos\brak{\frac{\theta_1}{2}}\\ \sin\brak{\frac{\theta_1}{2}}}
\\
\vec{C}-\vec{A}&= r\myvec{\cos \theta - 1 & \sin \theta  } 
\\
&= 2r \sin\brak{\frac{\theta}{2}} \myvec{-\sin\brak{\frac{\theta}{2}}\\ \cos\brak{\frac{\theta}{2}}}
\\
\implies \norm{\vec{D}-\vec{B}} &= 2r \cos\brak{\frac{\theta_1}{2}}
\\
\norm{\vec{C}-\vec{A}} &= 2r \sin\brak{\frac{\theta}{2}}\end{align}
Thus, using the definition of the inner product, 
\begin{align}
\cos \phase{E} &= \frac{ \brak{\vec{D}-\vec{B}}^T\brak{\vec{C}-\vec{A}} }{\norm{\vec{D}-\vec{B}}\norm{\vec{C}-\vec{A}}}
\\
&= \myvec{\cos\brak{\frac{\theta_1}{2}} & \sin\brak{\frac{\theta_1}{2}}} \myvec{-\sin\brak{\frac{\theta}{2}}\\ \cos\brak{\frac{\theta}{2}}}
\end{align}
which can be simplified to obtain
\begin{align}
\cos \phase{E} &=\sin\brak{\frac{\theta_1-\theta}{2}} 
\\
&= \sin 30\degree = \frac{1}{2}
\end{align}
from \eqref{eq:8.5.16_theta_diff}.  Thus, 
\begin{align}
\phase{E} = 60 \degree
\end{align}

