\renewcommand{\theequation}{\theenumi}
\begin{enumerate}[label=\arabic*.,ref=\thesubsection.\theenumi]
\numberwithin{equation}{enumi}

\item Draw quadrilateral $ABCD$ with 
\begin{align}
BC &= a = 4.5,  
CD = b = 5.5, 
AD c = 4,
\\  
AB &= d = 6,
BD = e = 7 
\end{align}
%
\begin{figure}[!ht]
	\begin{center}
			\resizebox{\columnwidth}{!}{\input{./figs/quad/quad_sss.tex}}
	\end{center}
	\caption{Drawing a quadrilateral given 4 sides and a diagonal}
	\label{fig:quad_sss}	
\end{figure}
%
\\
\solution The angles $\theta_1$ and $\theta_2$ in Fig. 	\ref{fig:quad_sss}	
are calculated using the cosine formula as
\begin{align}
\label{eq:tri_rot_ang}
\cos \theta_1 = \frac{a^2+e^2-b^2}{2ae}
\\
\cos \theta_2 = \frac{d^2+e^2-c^2}{2de}
\end{align}
%
The coordinates are then obtained as
\begin{multline}
\label{eq:tri_basic_new}
\vec{A} = d\myvec{\cos \brak{\theta_1+\theta_2}\\ \sin \brak{\theta_1+\theta_2}}, \vec{B} = \myvec{0\\0}, \vec{C} = \myvec{a\\0}, 
\\
\vec{D} = e\myvec{\cos \theta_1\\ \sin \theta_1}
\end{multline}
%
The python code for Fig. \ref{fig:quad_sss}	is available in 
%
\begin{lstlisting}
codes/quad/quad_sss.py
\end{lstlisting}
and the equivalent latex-tikz code is
%
\begin{lstlisting}
figs/quad/quad_sss.tex
\end{lstlisting}
%
\item Fig. 	\ref{fig:tri_rot} shows that the quadrilateral $ABCD$ can also be drawn by drawing $\triangle A_1BD_1$ and rotating it by $\theta_2$. Show that 

\begin{align}
\label{eq:tri_rot_trans}
\vec{D} = \vec{P}\vec{D}_1
\\
\vec{A} = \vec{P}\vec{A}_1
\end{align}
%
where 
\begin{align}
\label{eq:tri_rot_mat}
\vec{P} = \myvec{\cos\theta_2 & -\sin \theta_2\\ \sin \theta_2 & \cos \theta_2}
\end{align}
%
is known as the {\em rotation matrix}.
\begin{figure}[!ht]
	\begin{center}
			\resizebox{\columnwidth}{!}{\input{./figs/quad/tri_rot.tex}}
	\end{center}
	\caption{Drawing a quadrilateral given 4 sides and a diagonal}
	\label{fig:tri_rot}	
\end{figure}
%
\item Draw $\triangle ABC$ if $AB = 3, AC = 5$ and $\angle C = 30 \degree$.
%
\\
\solution From the cosine formula,
\begin{align}
\cos C = \frac{a^2+b^2-c^2}{2ab}
\end{align}
%
which can be expressed as
\begin{align}
\label{eq:quad_eq}
a^2 -2ab\cos C +b^2-c^2 = 0.
\end{align}
\begin{align}
\because \brak{a-b\cos C}^2 = a^2+b^2\cos^2C -2ab\cos C,
\end{align}
\eqref{eq:quad_eq} can be expressed as 
\begin{align}
\brak{a-b\cos C}^2 -b^2\cos^2C+b^2-c^2 = 0
\\
\implies \brak{a-b\cos C}^2 = b^2\brak{1-\cos^2C}-c^2
\\
\text{or}, a = b\cos C \pm \sqrt{b^2\brak{1-\cos^2C}-c^2}
\label{eq:tri_quad_sol}
\end{align}
%
Choose the value(s) for which $a > 0$.
\item The solution of a quadratic equation
\begin{align}
\label{eq:tri_quad_eq}
\alpha x^2 + \beta x + \gamma = 0
\end{align}
is given by 
\begin{align}
\label{eq:tri_quad_eq_sol}
x = \frac{-\beta \pm \sqrt{\beta^2 - 4\alpha\gamma}}{2\alpha}.
\end{align}
Verify \eqref{eq:tri_quad_sol} using \eqref{eq:tri_quad_eq_sol}.

\end{enumerate}
%
